src/base_logic/lib/ghost_map.v
@@ -2,11 +2,27 @@
 From iris.base_logic Require Export lib.ghost_map.
 
 (* Add some Perennial-specific stuff *)
+From iris.proofmode Require Import tactics.
 From Perennial.algebra Require Import own_discrete atleast.
 
 Section lemmas.
   Context `{ghost_mapG Σ K V}.
   Implicit Types (k : K) (v : V) (dq : dfrac) (q : Qp) (m : gmap K V).
+
+  (* FIXME upstream *)
+  Lemma ghost_map_insert_big {γ σ} σ' :
+    σ' ##ₘ σ →
+    ghost_map_auth γ 1 σ ==∗
+    ghost_map_auth γ 1 (σ' ∪ σ) ∗ ([∗ map] l ↦ v ∈ σ', l ↪[γ] v).
+  Proof using Type.
+    revert σ; induction σ' as [| l v σ' Hl IH] using map_ind; iIntros (σ Hdisj) "Hσ".
+    { rewrite left_id_L. auto. }
+    iMod (IH with "Hσ") as "[Hσ'σ Hσ']"; first by eapply map_disjoint_insert_l.
+    decompose_map_disjoint.
+    rewrite !big_opM_insert // -insert_union_l //.
+    by iMod (ghost_map_insert with "Hσ'σ") as "($ & $)";
+      first by apply lookup_union_None.
+  Qed.
 
   Global Instance ghost_map_auth_discrete γ q m : Discretizable (ghost_map_auth γ q m).
   Proof. rewrite ghost_map_auth_eq. apply _. Qed.
