src/program_proof/wal/circ_proof.v
@@ -1,6 +1,5 @@
 From iris.bi.lib Require Import fractional.
 From Perennial.base_logic.lib Require Import mono_nat.
-From Perennial.algebra Require Import deletable_heap.
 
 From RecordUpdate Require Import RecordSet.
 
