src/program_proof/wal/circ_proof_crash.v
@@ -1,5 +1,4 @@
 From iris.bi.lib Require Import fractional.
-From Perennial.algebra Require Import deletable_heap.
 From Perennial.goose_lang Require Import mono_nat.
 
 From RecordUpdate Require Import RecordSet.
